LambdaP/Lemmas/StoWeaken.lean
@@ -23,13 +23,13 @@ theorem Sub.sto_weaken {Θ Θ' : Sto} {Γ : Ctx s} {τ1 τ2 : Tau s}
   | .symm hw h1 => .symm (hw.sto_weaken hext) (h1.sto_weaken hext)
   | .fst_tm h1 => .fst_tm (h1.sto_weaken hext)
   | .fst_ty h1 => .fst_ty (h1.sto_weaken hext)
-  | .sel_tm hr hw h1 =>
-    .sel_tm hr (hw.sto_weaken hext) (h1.sto_weaken hext)
+  | .sel_tm hw h1 =>
+    .sel_tm (hw.sto_weaken hext) (h1.sto_weaken hext)
   | .sel_tm_loc hc hl => .sel_tm_loc (hc.sto_weaken hext) (hext hl)
-  | .sel_hi hr hw h1 h2 =>
-    .sel_hi hr (hw.sto_weaken hext) (h1.sto_weaken hext) (h2.sto_weaken hext)
-  | .sel_lo hr hw h1 h2 =>
-    .sel_lo hr (hw.sto_weaken hext) (h1.sto_weaken hext) (h2.sto_weaken hext)
+  | .sel_hi hw h1 h2 =>
+    .sel_hi (hw.sto_weaken hext) (h1.sto_weaken hext) (h2.sto_weaken hext)
+  | .sel_lo hw h1 h2 =>
+    .sel_lo (hw.sto_weaken hext) (h1.sto_weaken hext) (h2.sto_weaken hext)
   | .sel_hi_loc hc hl => .sel_hi_loc (hc.sto_weaken hext) (hext hl)
   | .sel_lo_loc hc hl => .sel_lo_loc (hc.sto_weaken hext) (hext hl)
   | .arrow h1 h2 => .arrow (h1.sto_weaken hext) (h2.sto_weaken hext)
@@ -39,10 +39,10 @@ theorem Sub.sto_weaken {Θ Θ' : Sto} {Γ : Ctx s} {τ1 τ2 : Tau s}
   | .repl hwp hwq h1 h2 =>
     .repl (hwp.sto_weaken hext) (hwq.sto_weaken hext)
       (h1.sto_weaken hext) (h2.sto_weaken hext)
-  | .skip_tm hr hw h1 hne =>
-    .skip_tm hr (hw.sto_weaken hext) (h1.sto_weaken hext) hne
-  | .skip_ty hr hw h1 =>
-    .skip_ty hr (hw.sto_weaken hext) (h1.sto_weaken hext)
+  | .skip_tm hw h1 hne =>
+    .skip_tm (hw.sto_weaken hext) (h1.sto_weaken hext) hne
+  | .skip_ty hw h1 =>
+    .skip_ty (hw.sto_weaken hext) (h1.sto_weaken hext)
   | .skip_tm_loc hc hl hne => .skip_tm_loc (hc.sto_weaken hext) (hext hl) hne
   | .skip_ty_loc hc hl => .skip_ty_loc (hc.sto_weaken hext) (hext hl)
 
